@prefix rdf: <http://www.w3.org/1999/02/22-rdf-syntax-ns#>.
@prefix rdfs: <http://www.w3.org/2000/01/rdf-schema#>.
@prefix solid: <http://www.w3.org/ns/solid/terms#>.
@prefix foaf: <http://xmlns.com/foaf/0.1/>.
@prefix schema: <http:/schema.org/>.
@prefix ui: <http://www.w3.org/ns/ui#>.
@prefix vcard: <http://www.w3.org/2006/vcard/ns#>.
@prefix : <#>.

solid:User a rdfs:Class;
  rdfs:label "user"@en, "utilisateur"@fr;
  rdfs:comment """Any person who might use a Solid-based system""";
  rdfs:subClassOf foaf:Person, schema:Person, vcard:Individual.

# Since these options are opt-in, it is a bit strange to have new users opt in
# That they are new users - also we do not use this class for anything specific
# yet
# solid:NewUser a rdfs:Class;
#  rdfs:label "new user"@en;
#  rdfs:comment """A person who might use a Solid-based system who has a low
#  level of familiarity with technical details.""";
#  rdfs:subClassOf solid:User.

solid:PowerUser a rdfs:Class;
  rdfs:label "power user"@en;
  rdfs:comment """A person who might use a Solid-based system
  who is prepared to be given a more complex interface in order
  to be provided with more pwerful features.""";
  rdfs:subClassOf solid:User.

  solid:Developer a rdfs:Class;
    rdfs:label "Developer";
    rdfs:comment """Any person who might use a Solid-based system,
    who has software development skills.""";
    rdfs:subClassOf solid:User.
